pulse/lib/steel/pulse/Pulse.Readback.fst
@@ -1,69 +1,71 @@
 module Pulse.Readback
 module R = FStar.Reflection
 module L = FStar.List.Tot
-module T = FStar.Tactics
+// module T = FStar.Tactics
 module RT = FStar.Reflection.Typing
-open Pulse.Syntax
+open Pulse.Syntax.Base
 open Pulse.Reflection.Util
 open Pulse.Elaborate.Pure
 
-let (let?) (f:option 'a) (g:'a -> T.Tac (option 'b)) : T.Tac (option 'b) =
+let (let?) (f:option 'a) (g:'a -> option 'b) : option 'b =
   match f with
   | None -> None
   | Some x -> g x
 
-let rec readback_universe (u:R.universe)
-  : o:option universe{ Some? o ==> elab_universe (Some?.v o) == u } =
-  match R.inspect_universe u with
-  | R.Uv_Zero ->
-    Some U_zero
+// let rec readback_universe (u:R.universe)
+//   : o:option universe{ Some? o ==> elab_universe (Some?.v o) == u } =
+//   match R.inspect_universe u with
+//   | R.Uv_Zero ->
+//     Some U_zero
 
-  | R.Uv_Succ u' -> (
-    match readback_universe u' with
-    | None -> None
-    | Some u' -> 
-      Some (U_succ u')
-    )
+//   | R.Uv_Succ u' -> (
+//     match readback_universe u' with
+//     | None -> None
+//     | Some u' -> 
+//       Some (U_succ u')
+//     )
 
-  | R.Uv_Name (s, r) ->
-    assume (r == FStar.Reflection.Typing.Builtins.dummy_range);
-    Some (U_var s)
+//   | R.Uv_Name (s, r) ->
+//     assume (r == FStar.Reflection.Typing.Builtins.dummy_range);
+//     Some (U_var s)
 
-  | R.Uv_Max [u1; u2] -> (
-    assume (u2 << u);     //??
-    let u1' = readback_universe u1 in
-    let u2' = readback_universe u2 in
-    match u1', u2' with
-    | Some u1', Some u2' ->
-      Some (U_max u1' u2')
-    | _ -> None
-    )
+//   | R.Uv_Max [u1; u2] -> (
+//     assume (u2 << u);     //??
+//     let u1' = readback_universe u1 in
+//     let u2' = readback_universe u2 in
+//     match u1', u2' with
+//     | Some u1', Some u2' ->
+//       Some (U_max u1' u2')
+//     | _ -> None
+//     )
 
-  | _ -> None
+//   | _ -> None
 
-let rec readback_universes (us:list R.universe)
-  : o:option (list universe) { 
-          Some? o ==> List.Tot.map elab_universe (Some?.v o) == us 
-    }
-  = match us with
-    | [] -> Some []
-    | hd::tl -> 
-      match readback_universe hd with
-      | None -> None
-      | Some hd -> 
-        match readback_universes tl with
-        | None -> None
-        | Some tl -> Some (hd::tl)
+// let rec readback_universes (us:list R.universe)
+//   : o:option (list universe) { 
+//           Some? o ==> List.Tot.map elab_universe (Some?.v o) == us 
+//     }
+//   = match us with
+//     | [] -> Some []
+//     | hd::tl -> 
+//       match readback_universe hd with
+//       | None -> None
+//       | Some hd -> 
+//         match readback_universes tl with
+//         | None -> None
+//         | Some tl -> Some (hd::tl)
     
 #push-options "--z3rlimit_factor 20"
+// TODO: FIXME: may be mark as opaque_to_smt
 let try_readback_st_comp
   (t:R.term)
-  (readback_ty:(t':R.term -> T.Tac (option (ty:term { elab_term ty == t' }))))
+  (readback_ty:(t':R.term ->
+                option (ty:term { elab_term ty == t' })))
 
-  : T.Tac (option (c:comp{elab_comp c == t})) =
+  : option (c:comp{elab_comp c == t}) =
 
   let open R in
-  let hd, args = T.collect_app t in
+  let hd, args = collect_app_ln t in
   match inspect_ln hd with
   | Tv_UInst fv [u] ->
     let fv_lid = inspect_fv fv in
@@ -79,7 +81,6 @@ let try_readback_st_comp
               assume (fv == stt_fv);
               assume (aq == Q_Explicit           /\
                       attrs == []                /\
-                      // bv_view.bv_ppname == "_"   /\
                       bv_view.bv_index == 0      /\
                       sort == fst res /\
                       snd res == Q_Explicit      /\
@@ -87,13 +88,11 @@ let try_readback_st_comp
                       snd post == Q_Explicit);
 
               assume (t == mk_stt_comp u (fst res) (fst pre) (mk_abs (fst res) R.Q_Explicit body));
-              let? u'' = readback_universe u in
               let? res' = readback_ty (fst res) in
               let? pre' = readback_ty (fst pre) in
               let? post' = readback_ty body in
-              let c = C_ST {u=u''; res=res'; pre=pre';post=post'} in
-              assume (elab_universe u'' == u);
-              Some (c <: c:Pulse.Syntax.comp{ elab_comp c == t })
+              let c = C_ST {u; res=res'; pre=pre';post=post'} in
+              Some (c <: c:Pulse.Syntax.Base.comp{ elab_comp c == t })
             | _ -> None)
          | _ -> None
     else if fv_lid = stt_atomic_lid || fv_lid = stt_ghost_lid
@@ -105,7 +104,6 @@ let try_readback_st_comp
                   = inspect_binder b
               in    
               let bv_view = inspect_bv bv in
-              let? u'' = readback_universe u in
               let? res' = readback_ty (fst res) in
               let? opened' = readback_ty (fst opened) in
               let? pre' = readback_ty (fst pre) in
@@ -113,15 +111,13 @@ let try_readback_st_comp
               if fv_lid = stt_atomic_lid
               then begin
                 assume (t == mk_stt_atomic_comp u (fst res) (fst opened) (fst pre) (mk_abs (fst res) R.Q_Explicit body));
-                let c = C_STAtomic opened' ({u=u''; res=res'; pre=pre';post=post'}) in
-                assume (elab_universe u'' == u);
-                Some (c <: c:Pulse.Syntax.comp{ elab_comp c == t })
+                let c = C_STAtomic opened' ({u; res=res'; pre=pre';post=post'}) in
+                Some (c <: c:Pulse.Syntax.Base.comp { elab_comp c == t })
               end
               else begin
                 assume (t == mk_stt_ghost_comp u (fst res) (fst opened) (fst pre) (mk_abs (fst res) R.Q_Explicit body));
-                let c = C_STGhost opened' ({u=u''; res=res'; pre=pre';post=post'}) in
-                assume (elab_universe u'' == u);
-                Some (c <: c:Pulse.Syntax.comp{ elab_comp c == t })
+                let c = C_STGhost opened' ({u; res=res'; pre=pre';post=post'}) in
+                Some (c <: c:Pulse.Syntax.Base.comp { elab_comp c == t })
               end
             | _ -> None)
          | _ -> None
@@ -133,18 +129,23 @@ let readback_qual = function
   | R.Q_Implicit -> Some Implicit
   | _ -> None
 
-let rec readback_ty (t:R.term)
-  : T.Tac (option (ty:term { elab_term ty == t })) =
+let collect_app_refined (t:R.term) : tuple2 (t':R.term{t' << t})
+                                            (list (a:R.argv{a << t})) =
+  admit ();
+  R.collect_app_ln t
 
-  let open T in
+#push-options "--z3rlimit 100 --fuel 4 --ifuel 4"
+let rec readback_ty (t:R.term)
+  : option (ty:term { elab_term ty == t }) =
+
   let open R in
-  let open Pulse.Syntax in
+  let open Pulse.Syntax.Base in
   
   match inspect_ln t with
   | Tv_Var bv ->
     let bv_view = inspect_bv bv in
     assume (bv_view.bv_index >= 0);
-    let r = Tm_Var {nm_index=bv_view.bv_index;nm_ppname=bv_view.bv_ppname;nm_range=range_of_term t} in
+    let r = tm_var {nm_index=bv_view.bv_index;nm_ppname=bv_view.bv_ppname;nm_range=range_of_term t} in
     // Needs some tweaks to how names are designed in the DSL,
     //   e.g. may need to expose ppname, what happens to tun bv sort?
     assume (elab_term r == t);
@@ -153,7 +154,7 @@ let rec readback_ty (t:R.term)
   | Tv_BVar bv ->
     let bv_view = inspect_bv bv in
     assume (bv_view.bv_index >= 0);
-    let r = Tm_BVar {bv_index=bv_view.bv_index;bv_ppname=bv_view.bv_ppname; bv_range=range_of_term t} in
+    let r = tm_bvar {bv_index=bv_view.bv_index;bv_ppname=bv_view.bv_ppname; bv_range=range_of_term t} in
     // Similar to the name case
     assume (elab_term r == t);
     Some r
@@ -168,15 +169,11 @@ let rec readback_ty (t:R.term)
     then Some Tm_Inames
     else if fv_lid = emp_inames_lid
     then Some Tm_EmpInames
-    else Some (Tm_FVar {fv_name=inspect_fv fv; fv_range=range_of_term t})
+    else Some (tm_fvar {fv_name=inspect_fv fv; fv_range=range_of_term t})
 
-  | Tv_UInst fv us -> (
+  | Tv_UInst fv us ->
     let fv = {fv_name=inspect_fv fv; fv_range=range_of_term t} in
-    match readback_universes us with
-    | None -> None
-    | Some us' -> Some (Tm_UInst fv us')
-    )
-
+    Some (tm_uinst fv us)
 
   | Tv_App hd (a, q) -> 
     let aux () = 
@@ -187,33 +184,31 @@ let rec readback_ty (t:R.term)
         let? arg' = readback_ty a in
         Some (Tm_PureApp hd' (readback_qual q) arg' <: ty:term {elab_term ty == t})
     in
-    let head, args = T.collect_app t in
+    let head, args = collect_app_refined t in
     begin
     match inspect_ln head, args with
-    | Tv_FVar fv, [(a1,_); (a2,_)] -> 
+    | Tv_FVar fv, [(a1, _); (a2, _)] ->
       if inspect_fv fv = star_lid
       then (
         let? t1 = readback_ty a1 in
         let? t2 = readback_ty a2 in
         assume (elab_term (Tm_Star t1 t2) == t);
-        Some #(t':Pulse.Syntax.term {elab_term t' == t}) (Tm_Star t1 t2)
+        Some #(t':Pulse.Syntax.Base.term {elab_term t' == t}) (Tm_Star t1 t2)
       )
       else aux ()
     | Tv_UInst fv [u], [(a1, _); (a2, _)] ->
       if inspect_fv fv = exists_lid ||
          inspect_fv fv = forall_lid
       then (
-        let? u = readback_universe u in
         let? ty = readback_ty a1 in
         let? p =
           match inspect_ln a2 with
           | Tv_Abs _ body ->
             let? p = readback_ty body in
             Some p <: option term
-          | _ ->
-            T.fail "readback_ty: only lambda expressions allowed when reading back exists/forall" in
+          | _ -> None in  // TODO: FIXME: provide error from this function?
 
-        let pulse_t : (t':Pulse.Syntax.term{elab_term t' == t}) =
+        let pulse_t : (t':Pulse.Syntax.Base.term{elab_term t' == t}) =
           if inspect_fv fv = exists_lid
           then begin
             assume (elab_term (Tm_ExistsSL u ty p should_elim_true) == t);
@@ -232,7 +227,7 @@ let rec readback_ty (t:R.term)
       then (
         let? t1 = readback_ty a in
         assume (elab_term (Tm_Pure t1) == t);
-        Some #(t':Pulse.Syntax.term {elab_term t' == t}) (Tm_Pure t1)
+        Some #(t':Pulse.Syntax.Base.term {elab_term t' == t}) (Tm_Pure t1)
       )
       else aux ()
     | _ -> aux ()
@@ -242,64 +237,57 @@ let rec readback_ty (t:R.term)
     let bv_view = inspect_bv bv in
     let? ty = readback_ty sort in
     let? phi = readback_ty phi in
-    let r = Tm_Refine {binder_ty=ty;binder_ppname=bv_view.bv_ppname} phi in
+    let r = tm_refine {binder_ty=ty;binder_ppname=bv_view.bv_ppname} phi in
     assume (elab_term r == t);
     Some (r <: ty:term {elab_term ty == t})
 
   | Tv_Abs _ _ -> None  //T.fail "readback_ty: unexpected Tv_Abs"
 
-  | Tv_Arrow b c -> (
-    let { binder_bv=bv; binder_qual=aq; binder_attrs=attrs; binder_sort=sort } =
-        inspect_binder b
-    in
-    assume (attrs == []);
-    match aq with
-    | R.Q_Meta _ -> None
-    | _ -> 
-      let q = readback_qual aq in
-      RT.pack_inspect_binder b;  // This does not have SMTPat
-      let bv_view = inspect_bv bv in
-      assume (bv_view.bv_index == 0);
-      let c_view = inspect_comp c in
-      (match c_view with
-       | C_Total c_t ->
-         let? b_ty' = readback_ty sort in
-         let? c' = readback_comp c_t in
-         Some (Tm_Arrow {binder_ty=b_ty';binder_ppname=bv_view.bv_ppname} q c' <: ty:term{ elab_term ty == t})
-      | _ -> None)
-    )
+  | Tv_Arrow _ _ ->
+    Some (Tm_FStar t (range_of_term t))
+  // (
+  //   let { binder_bv=bv; binder_qual=aq; binder_attrs=attrs; binder_sort=sort } =
+  //       inspect_binder b
+  //   in
+  //   assume (attrs == []);
+  //   match aq with
+  //   | R.Q_Meta _ -> None
+  //   | _ -> 
+  //     let q = readback_qual aq in
+  //     RT.pack_inspect_binder b;  // This does not have SMTPat
+  //     let bv_view = inspect_bv bv in
+  //     assume (bv_view.bv_index == 0);
+  //     let c_view = inspect_comp c in
+  //     (match c_view with
+  //      | C_Total c_t ->
+  //        let? b_ty' = readback_ty sort in
+  //        let? c' = readback_comp c_t in
+  //        Some (tm_arrow {binder_ty=b_ty';binder_ppname=bv_view.bv_ppname} q c' <: ty:term{ elab_term ty == t})
+  //     | _ -> None)
+  //   )
 
-  | Tv_Type u -> (
-    match readback_universe u with
-    | None -> None
-    | Some u' -> Some (Tm_Type u' <: ty:term{ elab_term ty == t })
-    )
+  | Tv_Type _ -> Some (Tm_FStar t (range_of_term t))
 
-  | Tv_Const c ->
-    (match c with
-     | C_Unit -> Some (Tm_Constant Pulse.Syntax.Unit)
-     | C_True -> Some (Tm_Constant (Bool true))
-     | C_False -> Some (Tm_Constant (Bool false))
-     | C_Int n -> Some (Tm_Constant (Int n))
-     | _ -> T.fail "readback_ty: constant not supported")
+  | Tv_Const _ -> Some (Tm_FStar t (range_of_term t))
+ 
+  | Tv_Uvar _ _ -> None // TODO: FIXME: T.fail "readback_ty: unexpected Tv_Uvar"
 
-  | Tv_Uvar _ _ -> T.fail "readback_ty: unexpected Tv_Uvar"
+  | Tv_Let _ _ _ _ _ _ ->
+    Some (Tm_FStar t (range_of_term t))
+    // if recf
+    // then None // TODO: FIXME: T.fail "readback_ty: unexpected recursive Tv_Let"
+    // else begin
+    //   assume (attrs == []);
+    //   let bv_view = inspect_bv bv in
+    //   assume (bv_view.bv_index == 0);
+    //   let? bv_t' = readback_ty ty in
+    //   let? def' = readback_ty def in
+    //   let? body' = readback_ty body in
+    //   FStar.Sealed.sealed_singl bv_view.bv_ppname RT.pp_name_default;
+    //   Some (Tm_Let bv_t' def' body' <: ty:term { elab_term ty == t })
+    // end
 
-  | Tv_Let recf attrs bv ty def body ->
-    if recf
-    then T.fail "readback_ty: unexpected recursive Tv_Let"
-    else begin
-      assume (attrs == []);
-      let bv_view = inspect_bv bv in
-      assume (bv_view.bv_index == 0);
-      let? bv_t' = readback_ty ty in
-      let? def' = readback_ty def in
-      let? body' = readback_ty body in
-      FStar.Sealed.sealed_singl bv_view.bv_ppname RT.pp_name_default;
-      Some (Tm_Let bv_t' def' body' <: ty:term { elab_term ty == t })
-    end
-
-  | Tv_Match _ _ _ -> Some (Tm_FStar t)
+  | Tv_Match _ _ _ -> Some (Tm_FStar t (range_of_term t))
 
   //
   // The following is dropping the ascription, which is not ideal
@@ -313,16 +301,17 @@ let rec readback_ty (t:R.term)
   //   ascribed, but that failed a couple of proofs in HACL* : (
   //
   | Tv_AscribedT t _ _ _
-  | Tv_AscribedC t _ _ _ -> admit (); Some (Tm_FStar t)
+  | Tv_AscribedC t _ _ _ -> admit (); Some (Tm_FStar t (range_of_term t))
 
   | Tv_Unknown ->
     Some Tm_Unknown
 
   | Tv_Unsupp ->
     None
-  
-and readback_comp (t:R.term)
-  : T.Tac (option (c:comp{ elab_comp c == t})) =
+#pop-options  
+
+let readback_comp (t:R.term)
+  : option (c:comp { elab_comp c == t }) =
 
   let ropt = try_readback_st_comp t readback_ty in
   match ropt with
