pulse/lib/steel/pulse/Pulse.Syntax.Printer.fsti
@@ -4,11 +4,11 @@ module R = FStar.Reflection
 module T = FStar.Tactics
 
 val name_to_string (f:R.name) : string
-val constant_to_string (c:constant) : string
+// val constant_to_string (c:constant) : string
 val univ_to_string (u:universe) : string
 val qual_to_string (q:option qualifier) : string
-val binder_to_string (b:binder) : T.Tac string
 val term_to_string (t:term) : T.Tac string
+val binder_to_string (b:binder) : T.Tac string
 val comp_to_string (c:comp) : T.Tac string
 val term_list_to_string (sep:string) (t:list term): T.Tac string
 val st_term_to_string (t:st_term) : T.Tac string
