pulse/lib/steel/pulse/Pulse.Syntax.Util.fst
@@ -1,0 +1,94 @@
+module Pulse.Syntax.Util
+
+module R = FStar.Reflection
+
+open Pulse.Syntax.Base
+open Pulse.Syntax.Naming
+open Pulse.Elaborate.Pure
+open Pulse.Readback
+
+// let is_fvar (t:term) (nm:R.name) : bool =
+//   match t with
+//   | Tm_FStar host_term _ ->
+//     (match R.inspect_ln host_term with
+//      | R.Tv_FVar fv -> R.inspect_fv fv = nm
+//      | _ -> false)
+//   | _ -> false
+
+let (let?) (f:option 'a) (g:'a -> option 'b) : option 'b =
+  match f with
+  | None -> None
+  | Some x -> g x
+
+let is_var (t:term) : option nm =
+  let open R in
+  match t with
+  | Tm_FStar host_term r ->
+    begin match R.inspect_ln host_term with
+          | R.Tv_Var bv ->
+            let bv_view = R.inspect_bv bv in
+            Some {nm_index=bv_view.bv_index;
+                  nm_ppname=bv_view.bv_ppname;
+                  nm_range=r}
+          | _ -> None
+    end
+  | _ -> None
+
+
+let is_fvar (t:term) : option (R.name & list universe) =
+  let open R in
+  match t with
+  | Tm_FStar host_term _ ->
+    begin match inspect_ln host_term with
+          | Tv_FVar fv -> Some (inspect_fv fv, [])
+          | Tv_UInst fv us -> Some (inspect_fv fv, us)
+          | _ -> None
+    end
+  | _ -> None
+
+let is_fvar_app (t:term) : option (R.name &
+                                   list universe &
+                                   option qualifier &
+                                   option term) =
+  match is_fvar t with
+  | Some (l, us) -> Some (l, us, None, None)
+  | None ->
+    match t with
+    | Tm_PureApp head q arg ->
+      begin match is_fvar head with
+            | Some (l, us) -> Some (l, us, q, Some arg)
+            | None -> None
+      end
+    | _ -> None
+
+let is_arrow (t:term) : option (binder & option qualifier & comp) =
+  match t with
+  | Tm_FStar host_term _ ->
+    begin match R.inspect_ln host_term with
+          | R.Tv_Arrow b c ->
+            let {binder_bv;binder_qual;binder_sort} =
+              R.inspect_binder b in
+            begin match binder_qual with
+                  | R.Q_Meta _ -> None
+                  | _ ->
+                    let q = readback_qual binder_qual in
+                    let bv_view = R.inspect_bv binder_bv in
+                    let c_view = R.inspect_comp c in
+                    begin match c_view with
+                          | R.C_Total c_t ->
+                            let? binder_ty = readback_ty binder_sort in
+                            let? c =
+                              match readback_comp c_t with
+                              | Some c -> Some c <: option Pulse.Syntax.Base.comp
+                              | None -> None in
+                            Some ({binder_ty;
+                                   binder_ppname=bv_view.bv_ppname},
+                                  q,
+                                  c)
+                          | _ -> None
+                    end
+            end
+          
+          | _ -> None
+    end
+  | _ -> None
